ulib/prims.fst
@@ -107,15 +107,15 @@ let pure_wp   (a:Type) = pure_post a -> GTot pure_pre
 assume type guard_free: Type0 -> Type0
 
 inline let pure_return (a:Type) (x:a) (p:pure_post a) =
-     p x
+     forall (y:a). y==x ==> p y
 
 inline let pure_bind_wp (r1:range) (a:Type) (b:Type)
                    (wp1:pure_wp a) (wp2: (a -> GTot (pure_wp b)))
                    (p : pure_post b) =
-     labeled r1 "push" unit 
-     /\ wp1 (fun (x:a) -> 
-             labeled r1 "pop" unit 
-	     /\ wp2 x p)
+     (* labeled r1 "push" unit  *)
+     (* /\  *)wp1 (fun (x:a) -> 
+             (* labeled r1 "pop" unit  *)
+	     (* /\  *)wp2 x p)
 inline let pure_if_then_else (a:Type) (p:Type) (wp_then:pure_wp a) (wp_else:pure_wp a) (post:pure_post a) =
      l_ITE p (wp_then post) (wp_else post)
 
